seiostar/QTypes.fst
@@ -9,46 +9,49 @@ open IOStar
 [@@no_auto_projectors] // FStarLang/FStar#3986
 noeq
 type type_quotation : Type0 -> Type u#1 =
-| QUnit : type_quotation unit
-| QBool : type_quotation bool
-| QFileDescriptor : type_quotation file_descr
-| QString : type_quotation string
+| QUnit : #ref:(unit -> Type0) -> type_quotation (x:unit{ref x})
+| QBool : #ref:(bool -> Type0) -> type_quotation (x:bool{ref x})
+| QFileDescriptor : #ref:(file_descr -> Type0) -> type_quotation (x:file_descr{ref x})
+| QString : #ref:(string -> Type0) -> type_quotation (x:string{ref x})
 | QArr : #t1:Type ->
          #t2:Type ->
          type_quotation t1 ->
          type_quotation t2 ->
-         type_quotation (t1 -> t2)
+         #ref:((t1 -> t2) -> Type0) ->
+         type_quotation (f:(t1 -> t2){ref f})
 | QArrIO : #t1:Type ->
          #t2:Type ->
          type_quotation t1 ->
          type_quotation t2 ->
-         type_quotation (t1 -> io t2)
+         #ref:((t1 -> io t2) -> Type0) ->
+         type_quotation (f:(t1 -> io t2){ref f})
 | QPair : #t1:Type ->
           #t2:Type ->
           type_quotation t1 ->
           type_quotation t2 ->
-          type_quotation (t1 & t2)
+          #ref:(t1 & t2 -> Type0) ->
+          type_quotation (x:(t1 & t2){ref x})
 | QSum  : #t1:Type ->
           #t2:Type ->
           type_quotation t1 ->
           type_quotation t2 ->
-          type_quotation (either t1 t2)
-| QRefinement : #t:Type -> 
-                type_quotation t -> 
-                ref: (t -> Type0) ->
-                type_quotation (x:t{ref x})
-                
+          #ref:(either t1 t2 -> Type0) ->
+          type_quotation (x:(either t1 t2){ref x})
+// | QRefinement : #t:Type ->
+//                 type_quotation t ->
+//                 ref: (t -> Type0) ->
+//                 type_quotation (x:t{ref x})
+
 let test_match t (tq:type_quotation t) = (** why does this work so well? **)
   match tq with
-  | QUnit -> assert (t == unit)
-  | QBool -> assert (t == bool)
-  | QFileDescriptor -> assert (t == file_descr)
-  | QString -> assert (t == string)
-  | QArr #t1 #t2 _ _ -> assert (t == (t1 -> t2))
-  | QArrIO #t1 #t2 _ _ -> assert (t == (t1 -> io t2))
-  | QPair #t1 #t2 _ _ -> assert (t == (t1 & t2))
-  | QSum #t1 #t2 _ _ -> assert (t == either t1 t2)
-  | QRefinement #t' _ ref -> assert (x:t'{ref x} == t)
+  | QUnit #ref -> assert (t == x:unit{ref x})
+  | QBool #ref -> assert (t == x:bool{ref x})
+  | QFileDescriptor #ref -> assert (t == x:file_descr{ref x})
+  | QString #ref -> assert (t == x:string{ref x})
+  | QArr #t1 #t2 _ _ #ref -> assert (t == (f:(t1 -> t2){ref f}))
+  | QArrIO #t1 #t2 _ _ #ref -> assert (t == (f:(t1 -> io t2){ref f}))
+  | QPair #t1 #t2 _ _ #ref -> assert (t == (x:(t1 & t2){ref x}))
+  | QSum #t1 #t2 _ _ #ref -> assert (t == (x:(either t1 t2){ref x}))
 
 let rec type_quotation_to_typ #s (qt:type_quotation s) : typ =
   match qt with
@@ -61,7 +64,6 @@ let rec type_quotation_to_typ #s (qt:type_quotation s) : typ =
   | QArrIO qt1 qt2 ->
     TArr (type_quotation_to_typ qt1) (type_quotation_to_typ qt2)
   | QSum qt1 qt2 -> TSum (type_quotation_to_typ qt1) (type_quotation_to_typ qt2)
-  | QRefinement #t qt ref -> (type_quotation_to_typ qt)
 
 (** Type of Quotable Types **)
 type qType =
@@ -73,21 +75,29 @@ let get_Type (t:qType) = Mkdtuple2?._1 t
 let get_rel (t:qType) = Mkdtuple2?._2 t
 let lem_pack_get_rel t : Lemma (pack (get_rel t) == t) = ()
 
-let qUnit : qType = (| _, QUnit |)
-let qBool : qType = (| _, QBool |)
-let qFileDescr : qType = (| _, QFileDescriptor |)
-let qString : qType = (| _, QString |)
-let qRef (t:qType) (ref: get_Type t -> Type0) : qType =
-  (| _, QRefinement (get_rel t) ref |)
-let (^->) (t1 t2:qType) : qType =
-  (| _, QArr (get_rel t1) (get_rel t2) |)
-let (^->!@) (t1 t2:qType) : qType =
-  (| _, QArrIO (get_rel t1) (get_rel t2) |)
+let subQtype_of (a b:qType) : Type0 =
+  get_Type a `subtype_of` get_Type b
 
+let qUnitR ref : qType = (| _, QUnit #ref |)
+let qBoolR ref : qType = (| _, QBool #ref |)
+let qFileDescrR ref : qType = (| _, QFileDescriptor #ref |)
+let qStringR ref : qType = (| _, QString #ref |)
+
+let qUnit : qType = qUnitR (fun _ -> True)
+let qBool : qType = qBoolR (fun _ -> True)
+let qFileDescr : qType = qFileDescrR (fun _ -> True)
+let qString : qType = qStringR (fun _ -> True)
+
+// let qRef (t:qType) (ref: get_Type t -> Type0) : qType =
+//   (| _, QRefinement (get_rel t) ref |)
+let (^->) (t1 t2:qType) : qType =
+  (| _, QArr (get_rel t1) (get_rel t2) #(fun _ -> True) |)
+let (^->!@) (t1 t2:qType) : qType =
+  (| _, QArrIO (get_rel t1) (get_rel t2) #(fun _ -> True) |)
 let (^*) (t1 t2:qType) : qType =
-  (| _, QPair (get_rel t1) (get_rel t2) |)
+  (| _, QPair (get_rel t1) (get_rel t2) #(fun _ -> True) |)
 let (^+) (t1 t2:qType) : qType =
-  (| _, QSum (get_rel t1) (get_rel t2) |)
+  (| _, QSum (get_rel t1) (get_rel t2) #(fun _ -> True) |)
 
 let qResexn (t1:qType) : qType = t1 ^+ qUnit
 
